hol/p4_v1modelLib.sig
@@ -27,9 +27,9 @@ val v1model_func_map : term
 
 val dest_v1model_ascope : term -> term * term * term * term
 
-val dest_v1model_register_construct_inner : term -> term * term
+val dest_v1model_register_construct_inner : term -> term * term * term * term
 val is_v1model_register_construct_inner : term -> bool
-val mk_v1model_register_construct_inner : term * term -> term
+val mk_v1model_register_construct_inner : term * term * term * term -> term
 val v1model_register_construct_inner_tm : term
 
 val dest_v1model_register_read_inner : term -> term * term * term
