hol/p4_v1modelLib.sml
@@ -60,14 +60,14 @@ val v1model_apply_table_f = ``v1model_apply_table_f``;
 val v1model_ffblock_map = ``[("postparser", ffblock_ff v1model_postparser)]``;
 
 val v1model_register_map =
- ``[("read", ([("this", d_in); ("result", d_out); ("index", d_in)], register_read));
+ ``[("read", ([("this", d_in); ("result", d_out); ("index", d_in)], register_read random_oracle));
     ("write", ([("this", d_in); ("index", d_in); ("value", d_in)], register_write))]``;
 
 val v1model_ipsec_crypt_map =
- ``[("decrypt_aes_ctr", ([("this", d_in); ("ipv4", d_inout); ("esp", d_inout); ("standard_metadata", d_inout); ("key", d_in); ("key_hmac", d_in)], ipsec_crypt_decrypt_aes_ctr));
-    ("encrypt_aes_ctr", ([("this", d_in); ("ipv4", d_inout); ("esp", d_inout); ("key", d_in); ("key_hmac", d_in)], ipsec_crypt_encrypt_aes_ctr));
-    ("encrypt_null", ([("this", d_in); ("ipv4", d_inout); ("esp", d_inout)], ipsec_crypt_encrypt_null));
-    ("decrypt_null", ([("this", d_in); ("ipv4", d_inout); ("esp", d_inout); ("standard_metadata", d_inout)], ipsec_crypt_decrypt_null))]``;
+ ``[("decrypt_aes_ctr", ([("this", d_in); ("ipv4", d_inout); ("esp", d_inout); ("standard_metadata", d_inout); ("key", d_in); ("key_hmac", d_in)], ipsec_crypt_decrypt_aes_ctr random_oracle));
+    ("encrypt_aes_ctr", ([("this", d_in); ("ipv4", d_inout); ("esp", d_inout); ("key", d_in); ("key_hmac", d_in)], ipsec_crypt_encrypt_aes_ctr random_oracle));
+    ("encrypt_null", ([("this", d_in); ("ipv4", d_inout); ("esp", d_inout)], ipsec_crypt_encrypt_null random_oracle));
+    ("decrypt_null", ([("this", d_in); ("ipv4", d_inout); ("esp", d_inout); ("standard_metadata", d_inout)], ipsec_crypt_decrypt_null random_oracle))]``;
 
 (* Extern (object) function map *)
 val v1model_ext_map =
@@ -75,7 +75,7 @@ val v1model_ext_map =
     ++ [("", (NONE, (^v1model_objectless_map)));
         ("packet_in", (NONE, (^v1model_packet_in_map)));
         ("packet_out", (NONE, (^v1model_packet_out_map)));
-        ("register", SOME ([("this", d_out); ("size", d_none); ("targ1", d_in)], register_construct), (^v1model_register_map));
+        ("register", SOME ([("this", d_out); ("size", d_none); ("targ1", d_in)], register_construct random_oracle), (^v1model_register_map));
         ("ipsec_crypt", SOME ([("this", d_out)], ipsec_crypt_construct), (^v1model_ipsec_crypt_map))])``;
 
 (* Function map *)
@@ -95,7 +95,7 @@ fun dest_v1model_ascope v1model_ascope =
 ;
 
 val (v1model_register_construct_inner_tm,  mk_v1model_register_construct_inner, dest_v1model_register_construct_inner, is_v1model_register_construct_inner) =
-  syntax_fns2 "p4_v1model" "v1model_register_construct_inner";
+  syntax_fns4 "p4_v1model" "v1model_register_construct_inner";
 
 val (v1model_register_read_inner_tm,  mk_v1model_register_read_inner, dest_v1model_register_read_inner, is_v1model_register_read_inner) =
   syntax_fns3 "p4_v1model" "v1model_register_read_inner";
